# [&larr;](../index.md) Aula 17

## Exercício

![Exercício](../Images/86.jpeg)
![Q1](../Images/87.png)
![Q1-Youtube](../Images/90.png)
![Q2](../Images/88.png)
![Q3](../Images/89.png)

### Ex

Ex: f(x) = 2x - 2, xo = 1
Calcule f`(1)

Solução

f`(1) = lim((f(x) - f(1) / (x-1), x->1))

= lim((2x - 2) - (2*1 - 2) / (x - 1), x->1)

= lim((2x - 2) / x - 1, x->1)

= lim(2*(x - 1) / x - 1, x->1)

= 2

### Correção em Sala 27/05/2024

![Q1](../Images/91.jpeg)
![Q2](../Images/94.jpeg)
![Q3](../Images/95.jpeg)

### Exemplos em Sala

![ex1-pt1](../Images/92.jpeg)
![ex1-pt2](../Images/93.jpeg)

![ex2-pt1](../Images/96.jpeg)
![ex2-pt2](../Images/97.jpeg)

![ex3-pt1](../Images/98.jpeg)

![ex4-pt1](../Images/99.jpeg)
